clang/logic.v
@@ -1,0 +1,8 @@
+Require Import lang.
+
+Definition spec_state := nat. (* XXX: should be parameterized *)
+
+Definition spec_rel := spec_state → (option val * spec_state) → Prop.
+
+Inductive spec_code :=
+| SCrel : spec_rel → spec_code.
