clang/memory.v
@@ -1,0 +1,132 @@
+(** Definition of the physical memory model **)
+Require Export lib.Coqlib.
+Require Export Integers.
+Open Local Scope Z_scope.
+Require Import iris.base_logic.base_logic.
+
+Definition block : Set := positive.
+Definition offset := Z.
+Definition addr : Set := prod block offset.
+
+Instance addr_eq_dec : EqDecision addr.
+Proof. solve_decision. Defined.
+
+Inductive byteval : Set :=
+| BVundef
+| BVint8 (i: int8)
+| BVaddr (p: addr) (k: nat)
+| BVnull.
+
+(* (**Encoding and decoding for values**) *)
+(* Fixpoint encode_int (n: nat) (x: Z) {struct n}: list byte := *)
+(*   match n with *)
+(*     | O => nil *)
+(*     | S m => Byte.repr x :: encode_int m (x / 256) *)
+(*   end. *)
+
+(* Fixpoint decode_int (l: list byte): Z := *)
+(*   match l with *)
+(*     | nil => 0 *)
+(*     | b :: l' => Byte.unsigned b + decode_int l' * 256 *)
+(*   end. *)
+
+(* Lemma encode_int_length: *)
+(*   forall sz x, length(encode_int sz x) = sz. *)
+(* Proof. *)
+(*   induction sz; simpl; intros. auto. decEq. auto. *)
+(* Qed. *)
+
+(* Definition inj_bytes (bl: list byte) : list memval := *)
+(*   List.map Byte bl. *)
+
+(* Fixpoint proj_bytes (vl: list memval) : option (list byte) := *)
+(*   match vl with *)
+(*     | nil => Some nil *)
+(*     | Byte b :: vl' => *)
+(*       match proj_bytes vl' with None => None | Some bl => Some(b :: bl) end *)
+(*     | _ => None *)
+(*   end. *)
+
+(* Lemma length_inj_bytes: *)
+(*   forall bl, length (inj_bytes bl) = length bl. *)
+(* Proof. *)
+(*   intros. apply List.map_length. *)
+(* Qed. *)
+
+(* Lemma proj_inj_bytes: *)
+(*   forall bl, proj_bytes (inj_bytes bl) = Some bl. *)
+(* Proof. *)
+(*   induction bl; simpl. auto. rewrite IHbl. auto. *)
+(* Qed. *)
+
+(* Lemma inj_proj_bytes: *)
+(*   forall cl bl, proj_bytes cl = Some bl -> cl = inj_bytes bl. *)
+(* Proof. *)
+(*   induction cl; simpl; intros. *)
+(*   inv H; auto. *)
+(*   destruct a; try congruence. destruct (proj_bytes cl); inv H. *)
+(*   simpl. decEq. auto. *)
+(* Qed. *)
+
+(* Fixpoint inj_pointer (n: nat) (b: block) (ofs: int32) {struct n}: list memval := *)
+(*   match n with *)
+(*     | O => nil *)
+(*     | S m => Pointer b ofs m :: inj_pointer m b ofs *)
+(*   end. *)
+
+(* Fixpoint check_pointer (n: nat) (b: block) (ofs: int32) (vl: list memval) *)
+(*          {struct n} : bool := *)
+(*   match n, vl with *)
+(*     | O, nil => true *)
+(*     | S m, Pointer b' ofs' m' :: vl' => *)
+(*       peq b b' && Int.eq_dec ofs ofs' && beq_nat m m' && check_pointer m b ofs vl' *)
+(*     | _, _ => false *)
+(*   end. *)
+
+
+(* Definition proj_pointer (vl: list memval) : val := *)
+(*   match vl with *)
+(*     | Pointer b ofs n :: vl' => *)
+(*       if check_pointer 4%nat b ofs vl then Vptr (b, ofs) else Vundef *)
+(*     | _ => Vundef *)
+(*   end. *)
+
+(* Definition encode_val (t: type) (v: val) : list memval := *)
+(*   match v, t with *)
+(*   | Vint32  n, Tint8  => inj_bytes (encode_int 1%nat (Int.unsigned n)) *)
+(*   | Vint32  n, Tint16 => inj_bytes (encode_int 2%nat (Int.unsigned n)) *)
+(*   | Vint32  n, Tint32 => inj_bytes (encode_int 4%nat (Int.unsigned n)) *)
+(*   | Vptr (b, ofs), Tptr _ => inj_pointer 4%nat b (ofs) *)
+(*   | Vptr (b, ofs), Tcom_ptr _ => inj_pointer 4%nat b (ofs) *)
+(*   | Vnull, Tnull => list_repeat 4 MNull *)
+(*   | Vnull, Tptr _ => list_repeat 4 MNull *)
+(*   | Vnull, Tcom_ptr _ => list_repeat 4 MNull *)
+(*   | _, _ => list_repeat (typelen t) Undef *)
+(*   end. *)
+
+(* Definition decode_val (t: type) (vl: list memval) : val := *)
+(*   match proj_bytes vl with *)
+(*   | Some bl => *)
+(*       match t with *)
+(*       | Tint8  => Vint32(Int.zero_ext 8 (Int.repr (decode_int bl))) *)
+(*       | Tint16 => Vint32(Int.zero_ext 16 (Int.repr (decode_int bl))) *)
+(*       | Tint32 => Vint32(Int.repr(decode_int bl)) *)
+(*       | _ => Vundef *)
+(*       end *)
+(*   | None => *)
+(*     match vl with *)
+(*       | MNull :: MNull ::MNull :: MNull :: nil=> match t with *)
+(*                                  | Tnull => Vnull *)
+(*                                  | Tptr _ => Vnull *)
+(*                                  | Tcom_ptr _ => Vnull *)
+(*                                  | _ => Vundef *)
+(*                                end *)
+(*       | _ => *)
+(*         match t with *)
+(*           | Tptr _ => proj_pointer vl *)
+(*           | Tcom_ptr _ => proj_pointer vl *)
+(*           | _ => Vundef *)
+(*         end *)
+(*     end *)
+(*   end. *)
+
